qp/p1_categories/c3_wtypes/s1_exp.lean
@@ -11,7 +11,9 @@ open stdaux
 
 universe variables ℓobj ℓhom
 
-class HasExp {C : Cat.{ℓobj ℓhom}}
+/-! #brief An exponential object.
+-/
+class HasExp (C : Cat.{ℓobj ℓhom})
     (X Y : C^.obj)
 := (exp : C^.obj)
    (ev
@@ -28,10 +30,321 @@ class HasExp {C : Cat.{ℓobj ℓhom}}
        , e = ev ∘∘ finproduct.hom (univ Z e ↗ C^.id Y ↗↗))
    (uniq
      : ∀ [exp_Y_HasFinProduct : HasFinProduct C [exp, Y]]
-         (ev' : C^.hom (finproduct C [exp, Y]) X)
-         (ωev' : ∀ (Z : C^.obj) [Z_Y_HasFinProduct : HasFinProduct C [Z, Y]]
-                   (e : C^.hom (finproduct C [Z, Y]) X)
-                 , e = ev' ∘∘ finproduct.hom (univ Z e ↗ C^.id Y ↗↗))
-       , ev' = ev)
+         (Z : C^.obj) [Z_Y_HasFinProduct : HasFinProduct C [Z, Y]]
+         (e : C^.hom (finproduct C [Z, Y]) X)
+         (u : C^.hom Z exp)
+         (ωu : e = ev ∘∘ finproduct.hom (u ↗ C^.id Y ↗↗))
+       , u = univ Z e)
+
+/-! #brief A category with all exponential obejcts.
+-/
+class HasAllExp (C : Cat.{ℓobj ℓhom})
+:= (has_exp : ∀ (X Y : C^.obj), HasExp C X Y)
+
+instance HasAllExp.HasExp {C : Cat.{ℓobj ℓhom}}
+    [C_HasAllExp : HasAllExp C]
+    (X Y : C^.obj)
+    : HasExp C X Y
+:= HasAllExp.has_exp X Y
+
+/-! #brief A category which locally has all exponential obejcts.
+-/
+class HasAllLocalExp (C : Cat.{ℓobj ℓhom})
+:= (has_exp : ∀ (A : C^.obj) (X Y : (OverCat C A)^.obj)
+              , HasExp (OverCat C A) X Y)
+
+instance HasAllLocalExp.HasAllExp (C : Cat.{ℓobj ℓhom})
+    [C_HasAllLocalExp : HasAllLocalExp C]
+    (A : C^.obj)
+    : HasAllExp (OverCat C A)
+:= { has_exp := HasAllLocalExp.has_exp A
+   }
+
+/-! #brief An exponential object.
+-/
+definition expon (C : Cat.{ℓobj ℓhom})
+    (X Y : C^.obj)
+    [X_Y_HasExp : HasExp C X Y]
+    : C^.obj
+:= HasExp.exp X Y
+
+/-! #brief An evaluation map.
+-/
+definition expon.eval (C : Cat.{ℓobj ℓhom})
+    (X Y : C^.obj)
+    [X_Y_HasExp : HasExp C X Y]
+    [exp_Y_HasFinProduct : HasFinProduct C [expon C X Y, Y]]
+    : C^.hom (finproduct C [expon C X Y, Y]) X
+:= HasExp.ev X Y
+
+/-! #brief A universal map.
+-/
+definition expon.univ (C : Cat.{ℓobj ℓhom})
+    {X Y : C^.obj}
+    [X_Y_HasExp : HasExp C X Y]
+    {Z : C^.obj}
+    [Z_Y_HasFinProduct : HasFinProduct C [Z, Y]]
+    (e : C^.hom (finproduct C [Z, Y]) X)
+    : C^.hom Z (expon C X Y)
+:= HasExp.univ Z e
+
+/-! #brief The universal map factors.
+-/
+theorem expon.univ.factor {C : Cat.{ℓobj ℓhom}}
+    {X Y : C^.obj}
+    [X_Y_HasExp : HasExp C X Y]
+    [exp_Y_HasFinProduct : HasFinProduct C [expon C X Y, Y]]
+    {Z : C^.obj}
+    [Z_Y_HasFinProduct : HasFinProduct C [Z, Y]]
+    {e : C^.hom (finproduct C [Z, Y]) X}
+    : e = expon.eval C X Y ∘∘ finproduct.hom (expon.univ C e ↗ C^.id Y ↗↗)
+:= HasExp.factor Z e
+
+/-! #brief The universal map is unique.
+-/
+theorem expon.univ.uniq {C : Cat.{ℓobj ℓhom}}
+    {X Y : C^.obj}
+    [X_Y_HasExp : HasExp C X Y]
+    [exp_Y_HasFinProduct : HasFinProduct C [expon C X Y, Y]]
+    {Z : C^.obj} [Z_Y_HasFinProduct : HasFinProduct C [Z, Y]]
+    (e : C^.hom (finproduct C [Z, Y]) X)
+    (u : C^.hom Z (expon C X Y))
+    (ωu : e = expon.eval C X Y ∘∘ finproduct.hom (u ↗ C^.id Y ↗↗))
+    : u = expon.univ C e
+:= @HasExp.uniq C X Y X_Y_HasExp exp_Y_HasFinProduct Z Z_Y_HasFinProduct e u ωu
+
+/-! #brief The universal map induced by eval is the identity.
+-/
+theorem expon.univ_eval {C : Cat.{ℓobj ℓhom}}
+    {X Y : C^.obj}
+    [X_Y_HasExp : HasExp C X Y]
+    [exp_Y_HasFinProduct : HasFinProduct C [expon C X Y, Y]]
+    : C^.id (expon C X Y) = expon.univ C (expon.eval C X Y)
+:= expon.univ.uniq _ _ begin exact sorry end
+
+
+
+/- -----------------------------------------------------------------------
+Homs induce maps between exponentials.
+----------------------------------------------------------------------- -/
+
+/-! #brief Hom induced by composition on the right.
+-/
+definition expon.circ_right {C : Cat.{ℓobj ℓhom}}
+    {Z X Y : C^.obj}
+    [Z_X_HasExp : HasExp C Z X]
+    [Z_Y_HasExp : HasExp C Z Y]
+    [exp_Y_HasFinProduct : HasFinProduct C [expon C Z Y, Y]]
+    [exp_X_HasFinProduct : HasFinProduct C [expon C Z Y, X]]
+    (f : C^.hom X Y)
+    : C^.hom (expon C Z Y) (expon C Z X)
+:= expon.univ C (C^.circ (expon.eval C Z Y) (finproduct.hom (C^.id (expon C Z Y) ↗ f ↗↗)))
+
+/-! #brief Hom induced by composition on the left.
+-/
+definition expon.circ_left {C : Cat.{ℓobj ℓhom}}
+    {X Y Z : C^.obj}
+    [X_Z_HasExp : HasExp C X Z]
+    [Y_Z_HasExp : HasExp C Y Z]
+    [exp_Z_HasFinProduct : HasFinProduct C [expon C X Z, Z]]
+    (g : C^.hom X Y)
+    : C^.hom (expon C X Z) (expon C Y Z)
+:= expon.univ C (C^.circ g (expon.eval C X Z))
+
+/-! #brief Exponential objects are unique up-to unique isomorphism.
+-/
+definition expon.iso₁ {C : Cat.{ℓobj ℓhom}}
+    {X Y : C^.obj}
+    (X_Y_HasExp₁ X_Y_HasExp₂ : HasExp C X Y)
+    [exp_Y_HasFinProduct₁ : HasFinProduct C [@expon C X Y X_Y_HasExp₁, Y]]
+    : C^.hom (@expon C X Y X_Y_HasExp₁) (@expon C X Y X_Y_HasExp₂)
+:= @expon.circ_left C X X Y X_Y_HasExp₁ X_Y_HasExp₂ exp_Y_HasFinProduct₁ (C^.id X)
+
+/-! #brief Exponential objects are unique up-to unique isomorphism.
+-/
+definition expon.iso₂ {C : Cat.{ℓobj ℓhom}}
+    {X Y : C^.obj}
+    (X_Y_HasExp₁ X_Y_HasExp₂ : HasExp C X Y)
+    [exp_Y_HasFinProduct₂ : HasFinProduct C [@expon C X Y X_Y_HasExp₂, Y]]
+    : C^.hom (@expon C X Y X_Y_HasExp₂) (@expon C X Y X_Y_HasExp₁)
+:= @expon.circ_left C X X Y X_Y_HasExp₂ X_Y_HasExp₁ exp_Y_HasFinProduct₂ (C^.id X)
+
+/-! #brief Exponential objects are unique up-to unique isomorphism.
+-/
+definition expon.iso {C : Cat.{ℓobj ℓhom}}
+    {X Y : C^.obj}
+    (X_Y_HasExp₁ X_Y_HasExp₂ : HasExp C X Y)
+    [exp_Y_HasFinProduct₁ : HasFinProduct C [@expon C X Y X_Y_HasExp₁, Y]]
+    [exp_Y_HasFinProduct₂ : HasFinProduct C [@expon C X Y X_Y_HasExp₂, Y]]
+    : Iso (expon.iso₁ X_Y_HasExp₁ X_Y_HasExp₂)
+          (expon.iso₂ X_Y_HasExp₁ X_Y_HasExp₂)
+:= sorry
+
+
+
+/- -----------------------------------------------------------------------
+The exponential functor.
+----------------------------------------------------------------------- -/
+
+/-! #brief The exponential functor.
+-/
+definition ExpFun (C : Cat.{ℓobj ℓhom})
+    [C_HasAllExp : HasAllExp C]
+    [C_HasAllFinProducts : HasAllFinProducts C]
+    (W : C^.obj)
+    : Fun C C
+:= { obj := λ X, expon C X W
+   , hom := λ X Y f, expon.circ_left f
+   , hom_id := λ X
+               , begin
+                   dsimp [expon.circ_left],
+                   rw C^.circ_id_left,
+                   apply eq.symm expon.univ_eval
+                 end
+   , hom_circ
+      := λ X Y Z g f
+         , begin
+             dsimp [expon.circ_left],
+             refine eq.symm (expon.univ.uniq _ _ _),
+             refine eq.trans _
+                     (Cat.circ.congr_right
+                       (eq.trans 
+                         (eq.symm (finproduct.hom₂.circ
+                                    (expon.univ C (g ∘∘ expon.eval C Y W)) ⟨⟨W⟩⟩
+                                    (expon.univ C (f ∘∘ expon.eval C X W)) ⟨⟨W⟩⟩))
+                         (by rw C^.circ_id_right))),
+             refine eq.trans _ (eq.symm C^.circ_assoc),
+             refine eq.trans _ (Cat.circ.congr_left expon.univ.factor),
+             refine eq.trans (eq.symm C^.circ_assoc)
+                (eq.trans (Cat.circ.congr_right expon.univ.factor) C^.circ_assoc),
+           end
+   }
+
+
+
+/- -----------------------------------------------------------------------
+The dependent product functor.
+----------------------------------------------------------------------- -/
+
+/-! #brief The dependent product functor.
+-/
+definition HasAllExp.DepProdFun (C : Cat.{ℓobj ℓhom})
+    {B A : C^.obj} (f : C^.hom B A)
+    [C_HasAllExp : HasAllExp (OverCat C A)]
+    [C_HasAllFinProducts : HasAllFinProducts (OverCat C A)]
+    : Fun (OverCat C B) (OverCat C A)
+:= let f_obj : (OverCat C A)^.obj
+            := { obj := B, hom := f }
+in let codom_obj : (OverCat C B)^.obj → (OverCat C A)^.obj
+                := λ Q, { obj := Q^.obj
+                        , hom := C^.circ f Q^.hom
+                        }
+   in { obj := λ Q, (ExpFun (OverCat C A) f_obj)^.obj (codom_obj Q)
+   , hom := λ Q₁ Q₂ h, (ExpFun (OverCat C A) f_obj)^.hom
+                        { hom := h^.hom
+                        , triangle
+                           := begin
+                                dsimp [OverObj.down],
+                                rw -C^.circ_assoc,
+                                exact Cat.circ.congr_right h^.triangle
+                              end
+                        }
+   , hom_id
+      := λ Q
+         , eq.trans (congr_arg _ (OverHom.eq begin trivial end))
+                    (ExpFun (OverCat C A) f_obj)^.hom_id
+   , hom_circ
+      := λ Q₁ Q₂ Q₃ h g
+         , eq.trans (congr_arg _ (OverHom.eq begin trivial end))
+                    (ExpFun (OverCat C A) f_obj)^.hom_circ
+   }
+
+
+
+/-! #brief Counit of the adjunction between base change and dependent product.
+-/
+definition HasAllExp.BaseChange_DepProd.Adj.counit.com {C : Cat.{ℓobj ℓhom}}
+    {B A : C^.obj} (f : C^.hom B A)
+    [f_HasPullbacksAlong : HasPullbacksAlong C f]
+    [C_HasAllExp : HasAllExp (OverCat C A)]
+    [C_A_HasAllFinProducts : HasAllFinProducts (OverCat C A)]
+    : ∀ (Q : OverObj C B)
+      , OverHom C B
+          ((BaseChangeFun f □□ HasAllExp.DepProdFun C f)^.obj Q)
+          Q
+| (OverObj.mk Q h)
+:= { hom := (expon.eval (OverCat C A) (OverObj.mk Q (f ∘∘ h)) (OverObj.mk B f))^.hom
+             ∘∘ sorry
+   , triangle := sorry
+   }
+
+/-! #brief Counit of the adjunction between base change and dependent product.
+-/
+definition HasAllExp.BaseChange_DepProd.Adj.counit {C : Cat.{ℓobj ℓhom}}
+    {B A : C^.obj} (f : C^.hom B A)
+    [f_HasPullbacksAlong : HasPullbacksAlong C f]
+    [C_HasAllExp : HasAllExp (OverCat C A)]
+    [C_HasAllFinProducts : HasAllFinProducts (OverCat C A)]
+    : NatTrans (BaseChangeFun f □□ HasAllExp.DepProdFun C f)
+               (Fun.id (OverCat C B))
+:= { com := HasAllExp.BaseChange_DepProd.Adj.counit.com f
+   , natural := sorry
+   }
+
+
+/-! #brief Unit of the adjunction between base change and dependent product.
+-/
+definition HasAllExp.BaseChange_DepProd.Adj.unit.com {C : Cat.{ℓobj ℓhom}}
+    {B A : C^.obj} (f : C^.hom B A)
+    [f_HasPullbacksAlong : HasPullbacksAlong C f]
+    [C_HasAllExp : HasAllExp (OverCat C A)]
+    [C_HasAllFinProducts : HasAllFinProducts (OverCat C A)]
+    (Q : OverObj C A)
+    : OverHom C A
+        Q
+        ((HasAllExp.DepProdFun C f □□ BaseChangeFun f)^.obj Q)
+:= { hom := sorry
+   , triangle := sorry
+   }
+
+/-! #brief Unit of the adjunction between base change and dependent product.
+-/
+definition HasAllExp.BaseChange_DepProd.Adj.unit {C : Cat.{ℓobj ℓhom}}
+    {B A : C^.obj} (f : C^.hom B A)
+    [f_HasPullbacksAlong : HasPullbacksAlong C f]
+    [C_HasAllExp : HasAllExp (OverCat C A)]
+    [C_HasAllFinProducts : HasAllFinProducts (OverCat C A)]
+    : NatTrans (Fun.id (OverCat C A))
+               (HasAllExp.DepProdFun C f □□ BaseChangeFun f)
+:= { com := HasAllExp.BaseChange_DepProd.Adj.unit.com f
+   , natural := sorry
+   }
+
+
+/-! #brief Base change is adjoint to dependent product.
+-/
+definition HasAllExp.BaseChange_DepProd.Adj (C : Cat.{ℓobj ℓhom})
+    {B A : C^.obj} (f : C^.hom B A)
+    [f_HasPullbacksAlong : HasPullbacksAlong C f]
+    [C_HasAllExp : HasAllExp (OverCat C A)]
+    [C_HasAllFinProducts : HasAllFinProducts (OverCat C A)]
+    : Adj (BaseChangeFun f) (HasAllExp.DepProdFun C f)
+:= { counit := HasAllExp.BaseChange_DepProd.Adj.counit f
+   , unit := HasAllExp.BaseChange_DepProd.Adj.unit f
+   , id_left := sorry
+   , id_right := sorry
+   }
+
+
+-- /-! #brief Locally cartesian closed categories have dependent product.
+-- -/
+-- instance HasAllExp.HasDepProdFun (C : Cat.{ℓobj ℓhom})
+--     [C_HasAllLocalExp : HasAllLocalExp C]
+--     [C_HasAllPullbacks : HasAllPullbacks C]
+--     : HasDepProdFun C
+-- := { depprod := λ x y f, HasAllExp.DepProdFun C f
+--    , adj := λ x y f f_HasPullbacksAlong, begin end -- HasAllExp.BaseChange_DepProd.Adj C f
+--    }
+
 
 end qp
